\documentclass[10pt,a4paper]{book}
\usepackage[utf8]{inputenc}
\usepackage[english]{babel}
\usepackage{amsmath}
\usepackage{amsfonts}
\usepackage{amssymb}
\usepackage{graphicx}
\usepackage{physics}
\usepackage{stmaryrd}
\usepackage[left=2cm,right=2cm,top=2cm,bottom=2cm]{geometry}
\author{Marco Biroli}
\title{GR - Cosmology TDs}

\begin{document}
\maketitle

\chapter{TD 1}
\section{Transverse Doppler effect and aberration.}
\begin{enumerate}
\item ...
\item ...
\item ...
\end{enumerate}

\section{Relativistic invariants and conserved quantities.}

\begin{enumerate}
\item \begin{enumerate}
\item The four position is given by $\vec{x} = \begin{pmatrix}
ct \\ \vb{x}
\end{pmatrix}$ and we have that the proper time differential is given by: $\dd t = \gamma \dd \tau$. Hence the four velocity is given by:
\[
\vec{u} = \dv{\vec{x}}{t} = \gamma  \begin{pmatrix}
c\\ \vb{u}
\end{pmatrix}
\]
\item We have the simple relation $p^\mu = m u^\mu$. Which gives:
\[
\vec{p} = \begin{pmatrix}
\gamma m c \\ \gamma m \vb{u}
\end{pmatrix} = \begin{pmatrix}
\frac{E}{c} \\ \gamma m \vb{u}
\end{pmatrix}
\]
\item The invariant built from the momentum is given by:
\[
p_\mu p^\mu = \eta_{\mu,\nu} p^\mu p^\nu = -m^2 c^2
\]
Which gives:
\[
m^2 c^4 = E^2 - |\vec{p}|^2 c^2
\]
\end{enumerate}
\item \begin{enumerate}
\item The conserved physical quantities are the energy of the whole system and the momentum of the center of mass. Hence in other words the four momentum is conserved.
\item The photon will lose energy and hence it will have a lower frequency $\nu' < \nu$. The four-momenta are given by:
\[
p_{e0} = (m, 0, 0, 0), p_{p0} = (E_0, 0, 0, E_0)
\]
And after the collision by:
\[
p_{e1} = (E'', 0, p_y, p_z), p_{p1} = (E', 0, - E' \sin\theta, - E' \cos \theta) 
\]
\item  
\end{enumerate}
\end{enumerate}


\chapter{}

\chapter{}
\section{Covariant derivatives and Christoffel symbols}
\begin{enumerate}
\item \begin{enumerate}
\item We have that:
\[
J^\mu_{\mu'} J^{\mu'}_{\nu} = \pdv{x^{\mu}}{x^{\mu'}} \pdv{x^{\mu'}}{x^\nu} = \pdv{x^{\mu}}{x^\nu} = \delta_\nu^\mu
\]
\item We have that:
\[
\left(J_{\sigma'}^\mu J_\mu^{\mu'} \right)_{, \gamma} = \left(\delta_{\mu}^\mu \right)_{, \gamma} = 0 \Rightarrow J_{\sigma', \gamma}^\mu J_\mu^{\mu'} = - J_{\sigma'}^\mu J_{\mu, \gamma}^{\mu'}
\]
\end{enumerate}

\item \begin{enumerate}

\item We have that:
\[
\partial_{\mu'}\phi'(x') = \pdv{}{x^{\mu'}} \phi(x) = \pdv{x^\mu}{x^{\mu'}} \pdv{}{x^\mu} \phi(x) = J_{\mu'}^\mu \partial_\mu \phi(x)
\]
Hence it is a tensor. 

\item No.

\item We have:
\begin{align*}
\grad_{\mu'}A^{\nu'} = \partial_{\mu'}A^{\nu'} = J_{\mu'}^\mu J_{\nu}^{\nu'} ( \partial_{\mu} A^\nu + \Gamma_{\mu \rho}^\nu A^\rho) &\Leftrightarrow J_{\mu'}^\mu J_{\nu}^{\nu'} \partial_{\mu} A^{\mu} + J_{\mu'}^\mu J_{\nu, \mu'}^{\nu'} A^\nu = J_{\mu'}^\mu J_{\nu}^{\nu'} \partial_{\mu} A^\nu + J_{\mu'}^\mu J_{\nu'}^\nu \Gamma_{\mu \rho}^\nu A^\rho\\
&\Leftrightarrow (J_{\mu'}^\mu J_{\nu, \mu'}^{\nu'} - J_{\mu'}^\mu J_{\sigma}^{\nu'} \Gamma_{\mu \nu}^\sigma) A^\nu = 0
\end{align*}
Which gives the desired result.

\item The exchange of the lower indices changes nothing.

\item We consider the invariant quantity $B^\mu A_\mu$ then:
\[
\grad_\rho(A_\mu B^\mu) = \partial_\rho(A_\mu B^\mu) = (\partial_\rho A_\mu)B^\mu + A_\mu \partial_\rho B^\mu
\]
However we also have that:
\[
\grad_\rho(A_\mu B^\mu) = (\grad_\rho A_\mu) B^\mu + A_\mu \grad_\rho B^\mu = (\grad_\rho A_\mu) B^\mu + A_\mu \partial_\rho B^\mu + A_\mu \Gamma_{\rho v}^\mu B^\nu
\]
Now equating both sides we obtain:
\[
(\partial_\rho A_\mu) B^\mu = \Gamma_{\rho M}^{\sigma} B^\mu A_\sigma + \grad_\rho A_\mu B^\mu
\]
Which gives:
\[
\grad_\rho A_\mu = \partial_\rho A_\mu - \Gamma_{\rho \mu}^\sigma A_\sigma
\]

\end{enumerate}

\item \begin{enumerate}

\item We have that:
\[
\Gamma^{\rho'}_{\nu' \mu'} = \pdv{x^{\rho'}}{X^\alpha} \pdv[2]{X^\alpha}{x^{\mu'}}{x^{\nu'}} = 
\]

\item 

\end{enumerate}

\end{enumerate}

\section{Geodesics and the shortest path}
\begin{enumerate}

\item \begin{enumerate}

\item We have that:
\[
S = - m \int | \dd s | = - m \int \sqrt{ \dd s_\mu \dd s^\mu }  = - m \int \sqrt{ g_{\mu \nu} \dd s^\mu \dd s^\nu }
\]
Now notice that:
\[
\dd s = \dv{x}{\lambda} \dd \lambda
\]
Hence re-writing on top we obtain:
\[
S = - m \int \sqrt{ - g_{\mu \nu} \dot{x}^\mu \dot{x}^\nu } \dd \lambda
\]

\item The Euler-Lagrange equations are given by:
\[
\dv{}{\lambda} \pdv{\mathcal{L}}{\dot{x}} - \pdv{\mathcal{L}}{x} = \dv{}{\lambda} \pdv{\mathcal{L}}{\dot{x}} = \dv{}{\lambda} \frac{-g_{\mu \nu} \dot{x}^\mu}{2 \mathcal{L}} = 
\]

\end{enumerate}



\end{enumerate}


\end{document}